\documentclass{subfiles}

\begin{document}

we have:
\begin{align*}
z_t & = U h_{t-1} + Wx_t + b \\
h_t & = f(z_t) \\
\delta_{t,k} & = \frac{\partial \mathcal{L}_t}{\partial z_k}
\end{align*}

for $\frac{\partial \mathcal{L}}{\partial W}$:
\begin{align*}
\frac{\partial \mathcal{L}_t}{\partial W}
& = \frac{\partial z_t}{\partial W}
    \frac{\partial h_t}{\partial z_t}
    \frac{\partial \mathcal{L}_t}{\partial h_t} \\
& = \big( \frac{\partial h_{t-1}}{\partial W}
          \frac{\partial z_t}{\partial h_{t-1}}
          + x_t^T \big)
    \frac{\partial h_t}{\partial z_t}
    \frac{\partial \mathcal{L}_t}{\partial h_t} \\
& = \big( \frac{\partial z_{t-1}}{\partial W}
          \frac{\partial h_{t-1}}{\partial z_{t-1}}
          \frac{\partial z_t}{\partial h_{t-1}}
          + x_t^T \big)
    \frac{\partial h_t}{\partial z_t}
    \frac{\partial \mathcal{L}_t}{\partial z_t} \\
& = \frac{\partial z_{t-1}}{\partial W}
    \frac{\partial \mathcal{L}_t}{\partial z_{t-1}}
    + x^T_t \frac{\partial \mathcal{L}_t}{\partial z_t} \\
& = \frac{\partial z_{t-1}}{\partial W} \delta_{t,t-1}
    + x^T_t \delta_{t,t} \\
& = \sum^t_{k=1} x^T_k \delta_{t,k} \\
\frac{\partial \mathcal{L}}{\partial W}
& = \sum^T_{t=1} \sum^t_{k=1} x^T_k \delta_{t,k}
\end{align*}

for $\frac{\partial \mathcal{L}}{\partial b}$:
\begin{align*}
\frac{\partial \mathcal{L}_t}{\partial b}
& = \frac{\partial z_t}{\partial b}
    \frac{\partial h_t}{\partial z_t}
    \frac{\partial \mathcal{L}_t}{\partial h_t} \\
& = \big( \frac{\partial z_{t-1}}{\partial b}
          \frac{\partial h_{t-1}}{\partial z_{t-1}}
          \frac{\partial z_t}{\partial h_{t-1}}
          + I \big)
    \frac{\partial h_t}{\partial z_t}
    \frac{\partial \mathcal{L}_t}{\partial h_t} \\
& = \frac{\partial z_{t-1}}{\partial b} \delta_{t,t-1}
    + \delta_{t,t} \\
& = \sum^t_{k=1} \delta_{t,k} \\
\frac{\partial \mathcal{L}}{\partial b}
& = \sum^T_{t=1} \sum^t_{k=1} \delta_{t,k}
\end{align*}

\end{document}